WIP.

tls_codec/proofs/fstar/extraction/Tls_codec.Bundle.fst
@@ -50,7 +50,8 @@ val impl_10': Core.Cmp.t_Eq t_Error
 unfold
 let impl_10 = impl_10'
 
-let impl_13: Core.Clone.t_Clone t_Error = { f_clone = (fun x -> x) }
+let impl_13: Core.Clone.t_Clone t_Error =
+  { f_clone = (fun x -> x); f_clone_pre = (fun _ -> True); f_clone_post = (fun _ _ -> True) }
 
 [@@ FStar.Tactics.Typeclasses.tcinstance]
 let impl_1: Core.Fmt.t_Display t_Error =
@@ -67,16 +68,19 @@ let impl_1: Core.Fmt.t_Display t_Error =
     f_fmt
     =
     fun (self: t_Error) (f: Core.Fmt.t_Formatter) ->
+      let args:t_Array Core.Fmt.Rt.t_Argument (mk_usize 1) =
+        let list = [Core.Fmt.Rt.impl__new_debug #t_Error self] in
+        FStar.Pervasives.assert_norm (Prims.eq2 (List.Tot.length list) 1);
+        Rust_primitives.Hax.array_of_list 1 list
+      in
       let tmp0, out:(Core.Fmt.t_Formatter & Core.Result.t_Result Prims.unit Core.Fmt.t_Error) =
         Core.Fmt.impl_11__write_fmt f
-          (Core.Fmt.Rt.impl_2__new_v1 (mk_usize 1)
+          (Core.Fmt.Rt.impl_1__new_v1 (mk_usize 1)
               (mk_usize 1)
               (let list = [""] in
                 FStar.Pervasives.assert_norm (Prims.eq2 (List.Tot.length list) 1);
                 Rust_primitives.Hax.array_of_list 1 list)
-              (let list = [Core.Fmt.Rt.impl__new_debug #t_Error self <: Core.Fmt.Rt.t_Argument] in
-                FStar.Pervasives.assert_norm (Prims.eq2 (List.Tot.length list) 1);
-                Rust_primitives.Hax.array_of_list 1 list)
+              args
             <:
             Core.Fmt.t_Arguments)
       in
@@ -88,9 +92,43 @@ let impl_1: Core.Fmt.t_Display t_Error =
   }
 
 [@@ FStar.Tactics.Typeclasses.tcinstance]
-assume val impl: Core.Error.t_Error t_Error
+let impl: Core.Error.t_Error t_Error =
+  {
+    _super_1049815079118268934 = FStar.Tactics.Typeclasses.solve;
+    _super_15857421111036552015 = FStar.Tactics.Typeclasses.solve
+  }
+
 [@@ FStar.Tactics.Typeclasses.tcinstance]
-assume val impl_2: Core.Convert.t_From t_Error Std.Io.Error.t_Error 
+let impl_2: Core.Convert.t_From t_Error Std.Io.Error.t_Error =
+  {
+    f_from_pre = (fun (e: Std.Io.Error.t_Error) -> true);
+    f_from_post = (fun (e: Std.Io.Error.t_Error) (out: t_Error) -> true);
+    f_from
+    =
+    fun (e: Std.Io.Error.t_Error) ->
+      match Std.Io.Error.impl_Error__kind e <: Std.Io.Error.t_ErrorKind with
+      | Std.Io.Error.ErrorKind_UnexpectedEof  -> Error_EndOfStream <: t_Error
+      | _ ->
+        let args:t_Array Core.Fmt.Rt.t_Argument (mk_usize 1) =
+          let list = [Core.Fmt.Rt.impl__new_debug #Std.Io.Error.t_Error e] in
+          FStar.Pervasives.assert_norm (Prims.eq2 (List.Tot.length list) 1);
+          Rust_primitives.Hax.array_of_list 1 list
+        in
+        Error_DecodingError
+        (Core.Hint.must_use #Alloc.String.t_String
+            (Alloc.Fmt.format (Core.Fmt.Rt.impl_1__new_v1 (mk_usize 1)
+                    (mk_usize 1)
+                    (let list = ["io error: "] in
+                      FStar.Pervasives.assert_norm (Prims.eq2 (List.Tot.length list) 1);
+                      Rust_primitives.Hax.array_of_list 1 list)
+                    args
+                  <:
+                  Core.Fmt.t_Arguments)
+              <:
+              Alloc.String.t_String))
+        <:
+        t_Error
+  }
 
 /// The `Size` trait needs to be implemented by any struct that should be
 /// efficiently serialized.
@@ -100,9 +138,7 @@ class t_Size (v_Self: Type0) = {
   f_tls_serialized_len_pre:v_Self -> Type0;
   f_tls_serialized_len_post:v_Self -> usize -> Type0;
   f_tls_serialized_len:x0: v_Self
-    -> Prims.Pure usize
-        (f_tls_serialized_len_pre x0)
-        (fun result -> f_tls_serialized_len_post x0 result)
+    -> usize
 }
 
 /// The `Serialize` trait provides functions to serialize a struct or enum.
@@ -120,10 +156,10 @@ class t_Serialize (v_Self: Type0) = {
       (v_W & Core.Result.t_Result usize t_Error)
     -> Type0;
   f_tls_serialize:#v_W: Type0 -> {| i1: Std.Io.t_Write v_W |} -> x0: v_Self -> x1: v_W
-    -> Prims.Pure (v_W & Core.Result.t_Result usize t_Error)
-        (f_tls_serialize_pre #v_W #i1 x0 x1)
-        (fun result -> f_tls_serialize_post #v_W #i1 x0 x1 result)
+    -> (v_W & Core.Result.t_Result usize t_Error)
 }
+
+
 
 class t_SerializeDetached (v_Self: Type0) = {
   f_tls_serialize_detached_pre:v_Self -> Type0;
@@ -138,8 +174,85 @@ class t_SerializeDetached (v_Self: Type0) = {
 }
 
 [@@ FStar.Tactics.Typeclasses.tcinstance]
-assume val impl_3 (#v_T: Type0) (#[FStar.Tactics.Typeclasses.tcresolve ()] i1: t_Serialize v_T)
-    : t_SerializeDetached v_T 
+assume val write_vec: Std.Io.t_Write (Alloc.Vec.t_Vec Rust_primitives.Integers.u8
+            Alloc.Alloc.t_Global)
+
+[@@ FStar.Tactics.Typeclasses.tcinstance]
+let impl_3 (#v_T: Type0) (#[FStar.Tactics.Typeclasses.tcresolve ()] i1: t_Serialize v_T)
+    : t_SerializeDetached v_T =
+  {
+    f_tls_serialize_detached_pre = (fun (self: v_T) -> true);
+    f_tls_serialize_detached_post
+    =
+    (fun
+        (self: v_T)
+        (out1: Core.Result.t_Result (Alloc.Vec.t_Vec u8 Alloc.Alloc.t_Global) t_Error)
+        ->
+        true);
+    f_tls_serialize_detached
+    =
+    fun (self: v_T) ->
+      let buffer:Alloc.Vec.t_Vec u8 Alloc.Alloc.t_Global =
+        Alloc.Vec.impl__with_capacity #u8
+          (f_tls_serialized_len #v_T #i1._super_6186925850915422136 self <: usize)
+      in
+      let tmp0, out:(Alloc.Vec.t_Vec u8 Alloc.Alloc.t_Global & Core.Result.t_Result usize t_Error) =
+        f_tls_serialize #v_T
+          #FStar.Tactics.Typeclasses.solve
+          #(Alloc.Vec.t_Vec u8 Alloc.Alloc.t_Global)
+          self
+          buffer
+      in
+      let buffer:Alloc.Vec.t_Vec u8 Alloc.Alloc.t_Global = tmp0 in
+      match out <: Core.Result.t_Result usize t_Error with
+      | Core.Result.Result_Ok written ->
+        if written <>. (Alloc.Vec.impl_1__len #u8 #Alloc.Alloc.t_Global buffer <: usize)
+        then
+          let args:(usize & usize) =
+            written, Alloc.Vec.impl_1__len #u8 #Alloc.Alloc.t_Global buffer <: (usize & usize)
+          in
+          let args:t_Array Core.Fmt.Rt.t_Argument (mk_usize 2) =
+            let list =
+              [
+                Core.Fmt.Rt.impl__new_display #usize args._1;
+                Core.Fmt.Rt.impl__new_display #usize args._2
+              ]
+            in
+            FStar.Pervasives.assert_norm (Prims.eq2 (List.Tot.length list) 2);
+            Rust_primitives.Hax.array_of_list 2 list
+          in
+          Core.Result.Result_Err
+          (Error_EncodingError
+            (Core.Hint.must_use #Alloc.String.t_String
+                (Alloc.Fmt.format (Core.Fmt.Rt.impl_1__new_v1 (mk_usize 3)
+                        (mk_usize 2)
+                        (let list =
+                            [
+                              "Expected that ";
+                              " bytes were written but the output holds ";
+                              " bytes"
+                            ]
+                          in
+                          FStar.Pervasives.assert_norm (Prims.eq2 (List.Tot.length list) 3);
+                          Rust_primitives.Hax.array_of_list 3 list)
+                        args
+                      <:
+                      Core.Fmt.t_Arguments)
+                  <:
+                  Alloc.String.t_String))
+            <:
+            t_Error)
+          <:
+          Core.Result.t_Result (Alloc.Vec.t_Vec u8 Alloc.Alloc.t_Global) t_Error
+        else
+          Core.Result.Result_Ok buffer
+          <:
+          Core.Result.t_Result (Alloc.Vec.t_Vec u8 Alloc.Alloc.t_Global) t_Error
+      | Core.Result.Result_Err err ->
+        Core.Result.Result_Err err
+        <:
+        Core.Result.t_Result (Alloc.Vec.t_Vec u8 Alloc.Alloc.t_Global) t_Error
+  }
 
 /// The `SerializeBytes` trait provides a function to serialize a struct or enum.
 /// The trait provides one function:
@@ -170,7 +283,7 @@ class t_Deserialize (v_Self: Type0) = {
     -> Type0;
   f_tls_deserialize:#v_R: Type0 -> {| i1: Std.Io.t_Read v_R |} -> x0: v_R
     -> Prims.Pure (v_R & Core.Result.t_Result v_Self t_Error)
-        (f_tls_deserialize_pre #v_R #i1 x0)
+        (true)
         (fun result -> f_tls_deserialize_post #v_R #i1 x0 result)
 }
 
@@ -196,8 +309,58 @@ class t_DeserializeExact (v_Self: Type0) = {
 }
 
 [@@ FStar.Tactics.Typeclasses.tcinstance]
-assume val impl_4 (#v_T: Type0) (#[FStar.Tactics.Typeclasses.tcresolve ()] i1: t_Deserialize v_T)
-    : t_DeserializeExact v_T 
+assume val read_slice:Std.Io.t_Read (Rust_primitives.Arrays.t_Slice Rust_primitives.Integers.u8
+        )
+
+[@@ FStar.Tactics.Typeclasses.tcinstance]
+let impl_4 (#v_T: Type0) (#[FStar.Tactics.Typeclasses.tcresolve ()] i1: t_Deserialize v_T)
+    : t_DeserializeExact v_T =
+  {
+    f_tls_deserialize_exact_pre
+    =
+    (fun
+        (#iimpl_677085834_: Type0)
+        (#[FStar.Tactics.Typeclasses.tcresolve ()]
+          i3:
+          Core.Convert.t_AsRef iimpl_677085834_ (t_Slice u8))
+        (bytes: iimpl_677085834_)
+        ->
+        true);
+    f_tls_deserialize_exact_post
+    =
+    (fun
+        (#iimpl_677085834_: Type0)
+        (#[FStar.Tactics.Typeclasses.tcresolve ()]
+          i3:
+          Core.Convert.t_AsRef iimpl_677085834_ (t_Slice u8))
+        (bytes: iimpl_677085834_)
+        (out2: Core.Result.t_Result v_T t_Error)
+        ->
+        true);
+    f_tls_deserialize_exact
+    =
+    fun
+      (#iimpl_677085834_: Type0)
+      (#[FStar.Tactics.Typeclasses.tcresolve ()]
+        i3:
+        Core.Convert.t_AsRef iimpl_677085834_ (t_Slice u8))
+      (bytes: iimpl_677085834_)
+      ->
+      let bytes:t_Slice u8 =
+        Core.Convert.f_as_ref #iimpl_677085834_ #(t_Slice u8) #FStar.Tactics.Typeclasses.solve bytes
+      in
+      let tmp0, out1:(t_Slice u8 & Core.Result.t_Result v_T t_Error) =
+        f_tls_deserialize #v_T #FStar.Tactics.Typeclasses.solve #(t_Slice u8) bytes
+      in
+      let bytes:t_Slice u8 = tmp0 in
+      match out1 <: Core.Result.t_Result v_T t_Error with
+      | Core.Result.Result_Ok out ->
+        if ~.(Core.Slice.impl__is_empty #u8 bytes <: bool)
+        then
+          Core.Result.Result_Err (Error_TrailingData <: t_Error) <: Core.Result.t_Result v_T t_Error
+        else Core.Result.Result_Ok out <: Core.Result.t_Result v_T t_Error
+      | Core.Result.Result_Err err -> Core.Result.Result_Err err <: Core.Result.t_Result v_T t_Error
+  }
 
 /// The `DeserializeBytes` trait defines functions to deserialize a byte slice
 /// to a struct or enum. In contrast to [`Deserialize`], this trait operates
@@ -209,7 +372,7 @@ class t_DeserializeBytes (v_Self: Type0) = {
     -> Type0;
   f_tls_deserialize_bytes:x0: t_Slice u8
     -> Prims.Pure (Core.Result.t_Result (v_Self & t_Slice u8) t_Error)
-        (f_tls_deserialize_bytes_pre x0)
+        (true)
         (fun result -> f_tls_deserialize_bytes_post x0 result)
 }
 
@@ -223,14 +386,35 @@ class t_DeserializeExactBytes (v_Self: Type0) = {
 }
 
 [@@ FStar.Tactics.Typeclasses.tcinstance]
-assume val impl_5 (#v_T: Type0) (#[FStar.Tactics.Typeclasses.tcresolve ()] i1: t_DeserializeBytes v_T)
-    : t_DeserializeExactBytes v_T 
+let impl_5 (#v_T: Type0) (#[FStar.Tactics.Typeclasses.tcresolve ()] i1: t_DeserializeBytes v_T)
+    : t_DeserializeExactBytes v_T =
+  {
+    f_tls_deserialize_exact_bytes_pre = (fun (bytes: t_Slice u8) -> true);
+    f_tls_deserialize_exact_bytes_post
+    =
+    (fun (bytes: t_Slice u8) (out1: Core.Result.t_Result v_T t_Error) -> true);
+    f_tls_deserialize_exact_bytes
+    =
+    fun (bytes: t_Slice u8) ->
+      match
+        f_tls_deserialize_bytes #v_T #FStar.Tactics.Typeclasses.solve bytes
+        <:
+        Core.Result.t_Result (v_T & t_Slice u8) t_Error
+      with
+      | Core.Result.Result_Ok (out, remainder) ->
+        if ~.(Core.Slice.impl__is_empty #u8 remainder <: bool)
+        then
+          Core.Result.Result_Err (Error_TrailingData <: t_Error) <: Core.Result.t_Result v_T t_Error
+        else Core.Result.Result_Ok out <: Core.Result.t_Result v_T t_Error
+      | Core.Result.Result_Err err -> Core.Result.Result_Err err <: Core.Result.t_Result v_T t_Error
+  }
 
 /// A 3 byte wide unsigned integer type as defined in [RFC 5246].
 /// [RFC 5246]: https://datatracker.ietf.org/doc/html/rfc5246#section-4.4
 type t_U24 = | U24 : t_Array u8 (mk_usize 3) -> t_U24
 
-let impl_15: Core.Clone.t_Clone t_U24 = { f_clone = (fun x -> x) }
+let impl_15: Core.Clone.t_Clone t_U24 =
+  { f_clone = (fun x -> x); f_clone_pre = (fun _ -> True); f_clone_post = (fun _ _ -> True) }
 
 [@@ FStar.Tactics.Typeclasses.tcinstance]
 assume
@@ -275,22 +459,68 @@ let impl_6__from_be_bytes (bytes: t_Array u8 (mk_usize 3)) : t_U24 = U24 bytes <
 
 let impl_6__to_be_bytes (self: t_U24) : t_Array u8 (mk_usize 3) = self._0
 
-let f_from__impl_7__v_LEN: usize = Core.Mem.size_of #usize ()
+let f_from__impl_7__v_LEN: usize = mk_usize 8
 
 [@@ FStar.Tactics.Typeclasses.tcinstance]
-assume val impl_7: Core.Convert.t_From usize t_U24 
+let impl_7: Core.Convert.t_From usize t_U24 =
+  {
+    f_from_pre = (fun (value: t_U24) -> true);
+    f_from_post = (fun (value: t_U24) (out: usize) -> true);
+    f_from
+    =
+    fun (value: t_U24) ->
+      let usize_bytes:t_Array u8 (mk_usize 8) = Rust_primitives.Hax.repeat (mk_u8 0) (mk_usize 8) in
+      let usize_bytes:t_Array u8 (mk_usize 8) =
+        Rust_primitives.Hax.Monomorphized_update_at.update_at_range_from usize_bytes
+          ({ Core.Ops.Range.f_start = f_from__impl_7__v_LEN -! mk_usize 3 <: usize }
+            <:
+            Core.Ops.Range.t_RangeFrom usize)
+          (Core.Slice.impl__copy_from_slice #u8
+              (usize_bytes.[ {
+                    Core.Ops.Range.f_start = f_from__impl_7__v_LEN -! mk_usize 3 <: usize
+                  }
+                  <:
+                  Core.Ops.Range.t_RangeFrom usize ]
+                <:
+                t_Slice u8)
+              (value._0 <: t_Slice u8)
+            <:
+            t_Slice u8)
+      in
+      Core.Num.impl_usize__from_be_bytes usize_bytes
+  }
 
 let f_try_from__impl_8__v_LEN: usize = Core.Mem.size_of #usize ()
 
 [@@ FStar.Tactics.Typeclasses.tcinstance]
-assume val impl__from__primitives (#v_T: Type0) (#[FStar.Tactics.Typeclasses.tcresolve ()] i1: t_Size v_T)
-    : t_Size (Core.Option.t_Option v_T) 
+let impl__from__primitives (#v_T: Type0) (#[FStar.Tactics.Typeclasses.tcresolve ()] i1: t_Size v_T)
+    : t_Size (Core.Option.t_Option v_T) =
+  {
+    f_tls_serialized_len_pre = (fun (self: Core.Option.t_Option v_T) -> true);
+    f_tls_serialized_len_post = (fun (self: Core.Option.t_Option v_T) (out: usize) -> true);
+    f_tls_serialized_len
+    =
+    fun (self: Core.Option.t_Option v_T) ->
+      
+      (match self <: Core.Option.t_Option v_T with
+        | Core.Option.Option_Some v ->
+          f_tls_serialized_len #v_T #FStar.Tactics.Typeclasses.solve v <: usize
+        | Core.Option.Option_None  -> mk_usize 0)
+  }
 
 [@@ FStar.Tactics.Typeclasses.tcinstance]
-assume val impl_1__from__primitives
+let impl_1__from__primitives
       (#v_T: Type0)
       (#[FStar.Tactics.Typeclasses.tcresolve ()] i1: t_Size v_T)
-    : t_Size (Core.Option.t_Option v_T) 
+    : t_Size (Core.Option.t_Option v_T) =
+  {
+    f_tls_serialized_len_pre = (fun (self: Core.Option.t_Option v_T) -> true);
+    f_tls_serialized_len_post = (fun (self: Core.Option.t_Option v_T) (out: usize) -> true);
+    f_tls_serialized_len
+    =
+    fun (self: Core.Option.t_Option v_T) ->
+      f_tls_serialized_len #(Core.Option.t_Option v_T) #FStar.Tactics.Typeclasses.solve self
+  }
 
 [@@ FStar.Tactics.Typeclasses.tcinstance]
 let impl_2__from__primitives
@@ -298,7 +528,7 @@ let impl_2__from__primitives
       (#[FStar.Tactics.Typeclasses.tcresolve ()] i1: t_Serialize v_T)
     : t_Serialize (Core.Option.t_Option v_T) =
   {
-    _super_6186925850915422136 = FStar.Tactics.Typeclasses.solve;
+    _super_6186925850915422136 = impl__from__primitives #v_T #i1._super_6186925850915422136;
     f_tls_serialize_pre
     =
     (fun
@@ -409,7 +639,7 @@ let impl_3__from__primitives
       (#[FStar.Tactics.Typeclasses.tcresolve ()] i1: t_SerializeBytes v_T)
     : t_SerializeBytes (Core.Option.t_Option v_T) =
   {
-    _super_6186925850915422136 = FStar.Tactics.Typeclasses.solve;
+    _super_6186925850915422136 = impl__from__primitives #v_T #i1._super_6186925850915422136;
     f_tls_serialize_bytes_pre = (fun (self: Core.Option.t_Option v_T) -> true);
     f_tls_serialize_bytes_post
     =
@@ -425,7 +655,7 @@ let impl_3__from__primitives
       | Core.Option.Option_Some e ->
         let out:Alloc.Vec.t_Vec u8 Alloc.Alloc.t_Global =
           Alloc.Vec.impl__with_capacity #u8
-            ((f_tls_serialized_len #v_T #FStar.Tactics.Typeclasses.solve e <: usize) +! mk_usize 1
+            ((f_tls_serialized_len #v_T #i1._super_6186925850915422136 e <: usize) +! mk_usize 1
               <:
               usize)
         in
@@ -438,7 +668,7 @@ let impl_3__from__primitives
             Core.Result.t_Result (Alloc.Vec.t_Vec u8 Alloc.Alloc.t_Global) t_Error
           with
           | Core.Result.Result_Ok hoist9 ->
-            let out:Alloc.Vec.t_Vec u8 Alloc.Alloc.t_Global =
+            let out,_:(Alloc.Vec.t_Vec u8 Alloc.Alloc.t_Global)&(Alloc.Vec.t_Vec u8 Alloc.Alloc.t_Global) =
               Alloc.Vec.impl_1__append #u8 #Alloc.Alloc.t_Global out hoist9
             in
             Core.Result.Result_Ok out
@@ -469,7 +699,7 @@ let impl_4__from__primitives
       (#[FStar.Tactics.Typeclasses.tcresolve ()] i1: t_Serialize v_T)
     : t_Serialize (Core.Option.t_Option v_T) =
   {
-    _super_6186925850915422136 = FStar.Tactics.Typeclasses.solve;
+    _super_6186925850915422136 = i1._super_6186925850915422136;
     f_tls_serialize_pre
     =
     (fun
@@ -515,7 +745,7 @@ let impl_5__from__primitives
       (#[FStar.Tactics.Typeclasses.tcresolve ()] i1: t_SerializeBytes v_T)
     : t_SerializeBytes (Core.Option.t_Option v_T) =
   {
-    _super_6186925850915422136 = FStar.Tactics.Typeclasses.solve;
+    _super_6186925850915422136 = i1._super_6186925850915422136;
     f_tls_serialize_bytes_pre = (fun (self: Core.Option.t_Option v_T) -> true);
     f_tls_serialize_bytes_post
     =
@@ -534,7 +764,7 @@ let impl_5__from__primitives
 let impl_6 (#v_T: Type0) (#[FStar.Tactics.Typeclasses.tcresolve ()] i1: t_Deserialize v_T)
     : t_Deserialize (Core.Option.t_Option v_T) =
   {
-    _super_6186925850915422136 = FStar.Tactics.Typeclasses.solve;
+    _super_6186925850915422136 = i1._super_6186925850915422136;
     f_tls_deserialize_pre
     =
     (fun
@@ -599,11 +829,16 @@ let impl_6 (#v_T: Type0) (#[FStar.Tactics.Typeclasses.tcresolve ()] i1: t_Deseri
                 <:
                 (v_R & Core.Result.t_Result (Core.Option.t_Option v_T) t_Error))
           | _ ->
+            let args:t_Array Core.Fmt.Rt.t_Argument (mk_usize 1) =
+              let list = [Core.Fmt.Rt.impl__new_display #u8 (some_or_none.[ mk_usize 0 ] <: u8)] in
+              FStar.Pervasives.assert_norm (Prims.eq2 (List.Tot.length list) 1);
+              Rust_primitives.Hax.array_of_list 1 list
+            in
             bytes,
             (Core.Result.Result_Err
               (Error_DecodingError
                 (Core.Hint.must_use #Alloc.String.t_String
-                    (Alloc.Fmt.format (Core.Fmt.Rt.impl_2__new_v1 (mk_usize 2)
+                    (Alloc.Fmt.format (Core.Fmt.Rt.impl_1__new_v1 (mk_usize 2)
                             (mk_usize 1)
                             (let list =
                                 [
@@ -613,16 +848,7 @@ let impl_6 (#v_T: Type0) (#[FStar.Tactics.Typeclasses.tcresolve ()] i1: t_Deseri
                               in
                               FStar.Pervasives.assert_norm (Prims.eq2 (List.Tot.length list) 2);
                               Rust_primitives.Hax.array_of_list 2 list)
-                            (let list =
-                                [
-                                  Core.Fmt.Rt.impl__new_display #u8
-                                    (some_or_none.[ mk_usize 0 ] <: u8)
-                                  <:
-                                  Core.Fmt.Rt.t_Argument
-                                ]
-                              in
-                              FStar.Pervasives.assert_norm (Prims.eq2 (List.Tot.length list) 1);
-                              Rust_primitives.Hax.array_of_list 1 list)
+                            args
                           <:
                           Core.Fmt.t_Arguments)
                       <:
@@ -650,6 +876,9 @@ let impl_37: t_Size u8 =
     f_tls_serialized_len_post = (fun (self: u8) (out: usize) -> true);
     f_tls_serialized_len = fun (self: u8) -> mk_usize 1
   }
+
+[@@ FStar.Tactics.Typeclasses.tcinstance]
+assume val default_u8: Core.Default.t_Default Rust_primitives.Integers.u8
 
 [@@ FStar.Tactics.Typeclasses.tcinstance]
 let impl_31: t_Deserialize u8 =
@@ -785,7 +1014,7 @@ let impl_7__from__primitives
       (#[FStar.Tactics.Typeclasses.tcresolve ()] i1: t_DeserializeBytes v_T)
     : t_DeserializeBytes (Core.Option.t_Option v_T) =
   {
-    _super_6186925850915422136 = FStar.Tactics.Typeclasses.solve;
+    _super_6186925850915422136 = i1._super_6186925850915422136;
     f_tls_deserialize_bytes_pre = (fun (bytes: t_Slice u8) -> true);
     f_tls_deserialize_bytes_post
     =
@@ -829,10 +1058,15 @@ let impl_7__from__primitives
                 <:
                 Core.Result.t_Result (Core.Option.t_Option v_T & t_Slice u8) t_Error)
           | _ ->
+            let args:t_Array Core.Fmt.Rt.t_Argument (mk_usize 1) =
+              let list = [Core.Fmt.Rt.impl__new_display #u8 some_or_none] in
+              FStar.Pervasives.assert_norm (Prims.eq2 (List.Tot.length list) 1);
+              Rust_primitives.Hax.array_of_list 1 list
+            in
             Core.Result.Result_Err
             (Error_DecodingError
               (Core.Hint.must_use #Alloc.String.t_String
-                  (Alloc.Fmt.format (Core.Fmt.Rt.impl_2__new_v1 (mk_usize 2)
+                  (Alloc.Fmt.format (Core.Fmt.Rt.impl_1__new_v1 (mk_usize 2)
                           (mk_usize 1)
                           (let list =
                               [
@@ -842,15 +1076,7 @@ let impl_7__from__primitives
                             in
                             FStar.Pervasives.assert_norm (Prims.eq2 (List.Tot.length list) 2);
                             Rust_primitives.Hax.array_of_list 2 list)
-                          (let list =
-                              [
-                                Core.Fmt.Rt.impl__new_display #u8 some_or_none
-                                <:
-                                Core.Fmt.Rt.t_Argument
-                              ]
-                            in
-                            FStar.Pervasives.assert_norm (Prims.eq2 (List.Tot.length list) 1);
-                            Rust_primitives.Hax.array_of_list 1 list)
+                          args
                         <:
                         Core.Fmt.t_Arguments)
                     <:
@@ -1016,6 +1242,11 @@ let impl_45: t_Size u16 =
     f_tls_serialized_len_post = (fun (self: u16) (out: usize) -> true);
     f_tls_serialized_len = fun (self: u16) -> mk_usize 2
   }
+
+[@@ FStar.Tactics.Typeclasses.tcinstance]
+assume val def_u16: Core.Default.t_Default Rust_primitives.Integers.u16
+[@@ FStar.Tactics.Typeclasses.tcinstance]
+assume val def_u32: Core.Default.t_Default Rust_primitives.Integers.u32
 
 [@@ FStar.Tactics.Typeclasses.tcinstance]
 let impl_39: t_Deserialize u16 =
@@ -2276,7 +2507,7 @@ let impl_9__from__primitives
       (#[FStar.Tactics.Typeclasses.tcresolve ()] i3: t_Deserialize v_U)
     : t_Deserialize (v_T & v_U) =
   {
-    _super_6186925850915422136 = FStar.Tactics.Typeclasses.solve;
+    _super_6186925850915422136 = impl_12__from__primitives #v_T #v_U #i2._super_6186925850915422136 #i3._super_6186925850915422136;
     f_tls_deserialize_pre
     =
     (fun
@@ -2336,7 +2567,7 @@ let impl_10__from__primitives
       (#[FStar.Tactics.Typeclasses.tcresolve ()] i3: t_DeserializeBytes v_U)
     : t_DeserializeBytes (v_T & v_U) =
   {
-    _super_6186925850915422136 = FStar.Tactics.Typeclasses.solve;
+    _super_6186925850915422136 = impl_12__from__primitives #v_T #v_U #i2._super_6186925850915422136 #i3._super_6186925850915422136;
     f_tls_deserialize_bytes_pre = (fun (bytes: t_Slice u8) -> true);
     f_tls_deserialize_bytes_post
     =
@@ -2374,7 +2605,7 @@ let impl_11__from__primitives
       (#[FStar.Tactics.Typeclasses.tcresolve ()] i3: t_Serialize v_U)
     : t_Serialize (v_T & v_U) =
   {
-    _super_6186925850915422136 = FStar.Tactics.Typeclasses.solve;
+    _super_6186925850915422136 = impl_12__from__primitives #v_T #v_U #i2._super_6186925850915422136 #i3._super_6186925850915422136;
     f_tls_serialize_pre
     =
     (fun
@@ -2456,7 +2687,7 @@ let impl_13__from__primitives
       (#[FStar.Tactics.Typeclasses.tcresolve ()] i5: t_Deserialize v_V)
     : t_Deserialize (v_T & v_U & v_V) =
   {
-    _super_6186925850915422136 = FStar.Tactics.Typeclasses.solve;
+    _super_6186925850915422136 = impl_16__from__primitives #v_T #v_U #v_V #i3._super_6186925850915422136 #i4._super_6186925850915422136 #i5._super_6186925850915422136;
     f_tls_deserialize_pre
     =
     (fun
@@ -2528,7 +2759,7 @@ let impl_14__from__primitives
       (#[FStar.Tactics.Typeclasses.tcresolve ()] i5: t_DeserializeBytes v_V)
     : t_DeserializeBytes (v_T & v_U & v_V) =
   {
-    _super_6186925850915422136 = FStar.Tactics.Typeclasses.solve;
+    _super_6186925850915422136 = impl_16__from__primitives #v_T #v_U #v_V #i3._super_6186925850915422136 #i4._super_6186925850915422136 #i5._super_6186925850915422136;
     f_tls_deserialize_bytes_pre = (fun (bytes: t_Slice u8) -> true);
     f_tls_deserialize_bytes_post
     =
@@ -2581,7 +2812,7 @@ let impl_15__from__primitives
       (#[FStar.Tactics.Typeclasses.tcresolve ()] i5: t_Serialize v_V)
     : t_Serialize (v_T & v_U & v_V) =
   {
-    _super_6186925850915422136 = FStar.Tactics.Typeclasses.solve;
+    _super_6186925850915422136 = impl_16__from__primitives #v_T #v_U #v_V #i3._super_6186925850915422136 #i4._super_6186925850915422136 #i5._super_6186925850915422136;
     f_tls_serialize_pre
     =
     (fun
@@ -2892,7 +3123,7 @@ let impl_26 (#v_T: Type0) (#[FStar.Tactics.Typeclasses.tcresolve ()] i1: t_Size 
 let impl_27 (#v_T: Type0) (#[FStar.Tactics.Typeclasses.tcresolve ()] i1: t_Serialize v_T)
     : t_Serialize (Alloc.Boxed.t_Box v_T Alloc.Alloc.t_Global) =
   {
-    _super_6186925850915422136 = FStar.Tactics.Typeclasses.solve;
+    _super_6186925850915422136 = i1._super_6186925850915422136;
     f_tls_serialize_pre
     =
     (fun
@@ -2941,7 +3172,7 @@ let impl_27 (#v_T: Type0) (#[FStar.Tactics.Typeclasses.tcresolve ()] i1: t_Seria
 let impl_28 (#v_T: Type0) (#[FStar.Tactics.Typeclasses.tcresolve ()] i1: t_SerializeBytes v_T)
     : t_SerializeBytes (Alloc.Boxed.t_Box v_T Alloc.Alloc.t_Global) =
   {
-    _super_6186925850915422136 = FStar.Tactics.Typeclasses.solve;
+    _super_6186925850915422136 = i1._super_6186925850915422136;
     f_tls_serialize_bytes_pre = (fun (self: Alloc.Boxed.t_Box v_T Alloc.Alloc.t_Global) -> true);
     f_tls_serialize_bytes_post
     =
@@ -2967,7 +3198,7 @@ let impl_28 (#v_T: Type0) (#[FStar.Tactics.Typeclasses.tcresolve ()] i1: t_Seria
 let impl_29 (#v_T: Type0) (#[FStar.Tactics.Typeclasses.tcresolve ()] i1: t_Deserialize v_T)
     : t_Deserialize (Alloc.Boxed.t_Box v_T Alloc.Alloc.t_Global) =
   {
-    _super_6186925850915422136 = FStar.Tactics.Typeclasses.solve;
+    _super_6186925850915422136 = i1._super_6186925850915422136;
     f_tls_deserialize_pre
     =
     (fun
@@ -3013,7 +3244,7 @@ let impl_29 (#v_T: Type0) (#[FStar.Tactics.Typeclasses.tcresolve ()] i1: t_Deser
 let impl_30 (#v_T: Type0) (#[FStar.Tactics.Typeclasses.tcresolve ()] i1: t_DeserializeBytes v_T)
     : t_DeserializeBytes (Alloc.Boxed.t_Box v_T Alloc.Alloc.t_Global) =
   {
-    _super_6186925850915422136 = FStar.Tactics.Typeclasses.solve;
+    _super_6186925850915422136 = i1._super_6186925850915422136;
     f_tls_deserialize_bytes_pre = (fun (bytes: t_Slice u8) -> true);
     f_tls_deserialize_bytes_post
     =
