tls_codec/proofs/fstar/models/Zeroize.fsti
@@ -1,0 +1,16 @@
+module Zeroize
+#set-options "--fuel 0 --ifuel 1 --z3rlimit 15"
+open Core
+open FStar.Mul
+
+class t_Zeroize (v_Self: Type0) = {
+  (* [@@@ FStar.Tactics.Typeclasses.no_method]_super_4726684624731801277:Core.Marker.t_MetaSized
+  v_Self; *)
+  f_zeroize_pre:v_Self -> Type0;
+  f_zeroize_post:v_Self -> v_Self -> Type0;
+  f_zeroize:x0: v_Self
+    -> Prims.Pure v_Self
+        (f_zeroize_pre x0)
+        (fun result ->
+            f_zeroize_post x0 result)
+}
